Add some utilities in CBitvector including bv_conv

Common/CBitvector.v
@@ -1,16 +1,16 @@
 (** Unfortunately this development needs to support two kinds of bitvector.
     The module will attempt to provide smooth interoperability between the two *)
 
+Require Import Coq.Logic.Eqdep. (* <- This assumes UIP *)
 Require Import Lia.
+Require Import stdpp.decidable.
 Require Export stdpp.unstable.bitvector.
 Require Export stdpp.unstable.bitvector_tactics.
 Require Export bbv.Word.
 Require Import CBase.
 Require Import CBool.
-Require Import Coq.Logic.Eqdep. (* <- This assumes UIP *)
 
 From Hammer Require Import Tactics.
-
 
 (*** Dependent types stuff ***)
 
@@ -551,7 +551,106 @@ Definition bv_set_bit (i : N) {n : N} (b : bv n) : bv n :=
 Definition bv_unset_bit (i : N) {n : N} (b : bv n) : bv n :=
   bv_or b (bv_not (Z_to_bv n (bv_modulus i))).
 
+Program Definition bv_1 (n : N) := Z_to_bv n 1.
+Program Definition bv_m1 (n : N) := Z_to_bv n (-1).
+
+Definition bv_eqb {n : N} (bv1 bv2 : bv n) : bool := bool_decide (bv1 = bv2).
+Definition bv_neqb {n : N} (bv1 bv2 : bv n) : bool := bool_decide (bv1 ≠ bv2).
+Definition bv_redand {n : N} (bv : bv n) : bool := bv_eqb bv (bv_m1 n).
+Definition bv_redor {n : N} (bv : bv n) : bool := bv_neqb bv (bv_0 n).
+
+
+Definition bv_nand {n : N} (bv1 bv2 : bv n) : bv n := bv_and bv1 bv2 |> bv_not.
+Definition bv_nor {n : N} (bv1 bv2 : bv n) : bv n := bv_or bv1 bv2 |> bv_not.
+Definition bv_xnor {n : N} (bv1 bv2 : bv n) : bv n := bv_xor bv1 bv2 |> bv_not.
+
+Module BVDecidableType.
+
+  Definition U := N.
+  Definition eq_dec (x y:U) : {x = y} + {x <> y} := decide_rel (=) x y.
+
+End BVDecidableType.
+
+Module BVEqDep := Eqdep_dec.DecidableEqDep(BVDecidableType).
+
+Definition bv_conv {n m : N} (e : n = m) (b : bv n) : bv m :=
+  match e with
+  | eq_refl => b
+  end.
+
+Lemma bv_conv_simpl {n} (e : n = n) (b : bv n) :
+  bv_conv e b = b.
+Proof.
+  rewrite (BVEqDep.UIP_refl n e).
+  reflexivity.
+Qed.
+#[global] Hint Rewrite @bv_conv_simpl : bv_unfold.
+
+Lemma bv_conv_trans {n m p : N} (e : n = m) (e' : m = p) (b : bv n) :
+  b |> bv_conv e |> bv_conv e' = b |> bv_conv (eq_trans e e').
+Proof. naive_solver. Qed.
+
+Lemma bv_conv_sym {n m : N} (e : n = m) (bn : bv n) (bm : bv m) :
+  bn = bv_conv (symmetry e) bm <-> bv_conv e bn = bm.
+Proof. naive_solver. Qed.
+
+Global Instance bv_unfold_bv_conv n m (e : n = m) s w b z:
+  BvUnfold n s w b z → BvUnfold m s w (bv_conv e b) z.
+Proof. tcclean. naive_solver. Qed.
+
+(*** Extra bvn functions ***)
 
 Definition BVN (n : N) (val : Z) {wf: BvWf n val} : bvn := BV n val.
 
 #[global] Instance bvn_empty : Empty bvn := BVN 0 0.
+
+Definition bvn_eqb (bv1 bv2 : bvn) : bool := bool_decide (bv1 = bv2).
+Definition bvn_neqb (bv1 bv2 : bvn) : bool := bool_decide (bv1 ≠ bv2).
+Definition bvn_redand (x : bvn) : bool := x |> bvn_val |> bv_redand.
+Definition bvn_redor (x : bvn) : bool := x |> bvn_val |> bv_redor.
+
+
+Definition bvn_succ (x : bvn) : bvn := x |> bvn_val |> bv_succ.
+Definition bvn_pred (x : bvn) : bvn := x |> bvn_val |> bv_pred.
+Definition bvn_not (x : bvn) : bvn := x |> bvn_val |> bv_not.
+Definition bvn_opp (x : bvn) : bvn := x |> bvn_val |> bv_opp.
+
+Lemma bvn_not_type (x : bvn) : bvn_n (bvn_not x) = bvn_n x.
+  Proof. naive_solver. Qed.
+
+Definition bvn_extract (s l : N) (x : bvn) : bvn :=
+  x |> bvn_val |> bv_extract s l.
+
+Definition bvn_zero_extend (l : N) (x : bvn) : bvn :=
+  x |> bvn_val |> bv_zero_extend l.
+
+Definition bvn_sign_extend (l : N) (x : bvn) : bvn :=
+  x |> bvn_val |> bv_sign_extend l.
+
+Definition bvn_binop (f : forall {n : N}, bv n -> bv n -> bv n) (x y : bvn)
+    : option bvn :=
+  match decide (bvn_n x = bvn_n y) with
+  | left eq => Some (f (bv_conv eq (bvn_val x)) (bvn_val y) : bvn)
+  | right _ => None
+  end.
+
+
+
+Definition bvn_mul := bvn_binop (@bv_mul).
+Definition bvn_add := bvn_binop (@bv_add).
+Definition bvn_sub := bvn_binop (@bv_sub).
+Definition bvn_divu := bvn_binop (@bv_divu).
+Definition bvn_modu := bvn_binop (@bv_modu).
+Definition bvn_divs := bvn_binop (@bv_divs).
+Definition bvn_quots := bvn_binop (@bv_quots).
+Definition bvn_mods := bvn_binop (@bv_mods).
+Definition bvn_rems := bvn_binop (@bv_rems). (* Yay REMS! *)
+Definition bvn_shiftl := bvn_binop (@bv_shiftl).
+Definition bvn_shiftr := bvn_binop (@bv_shiftr).
+Definition bvn_ashiftr := bvn_binop (@bv_ashiftr).
+Definition bvn_and := bvn_binop (@bv_and).
+Definition bvn_or := bvn_binop (@bv_or).
+Definition bvn_xor := bvn_binop (@bv_xor).
+
+Definition bvn_concat (b1 b2 : bvn) : bvn :=
+  bv_concat (bvn_n b1 + bvn_n b2) (bvn_val b1) (bvn_val b2).
